WIP: recursive vmprop for secondaries

theories/logrel/logrel.v
@@ -86,8 +86,8 @@ Section logrel.
     (R0 @@ V0 ->r encode_hvc_func(Send) ∗ (∃ rx_state'', RX_state@ i := rx_state'') ∗ ∃ j p_rx l, ⌜j ≠ i⌝ ∗ RX@ j := p_rx ∗ RX_state{1/2}@j := Some(l,i)
                           ∗ (∃r1, R1 @@ V0 ->r r1 ∗ ⌜decode_vmid r1 = Some j⌝) ∗  R2 @@ V0 ->r l ∗ ∃ mem_rx, memory_page p_rx mem_rx).
 
-  Definition vmprop_zero p_rx : iProp Σ :=
-    ((∃ ps_na'' ps_acc'' trans'' ,
+  Definition vmprop_zero_pre (Ψ: PID -d> PID -d> (gmap Word transaction) -d> iPropO Σ) :PID -d> PID -d> iPropO Σ :=
+    λ p_tx p_rx, (∃ ps_na'' ps_acc'' trans'' ,
                            let ps_macc_trans'' := pages_in_trans (trans_memory_in_trans trans'') in
                            (* lower bound *)
                            i -@{1/2}A> ps_acc'' ∗
@@ -103,15 +103,18 @@ Section logrel.
                            (* RX *)
                            rx_page i p_rx ∗ (∃ mem_rx, memory_page p_rx mem_rx) ∗
                            rx_pages ((list_to_set (list_of_vmids)) ∖ {[i]}) ∗
-                           return_reg_rx i)
-                           (* we don't give VMProp of i back, so there is no way to schedule i again. *)
-    ).
+                           return_reg_rx i ∗
+                           VMProp i (Ψ p_tx p_rx trans'') (1/2)%Qp)%I.
 
-  Definition vmprop_unknown p_tx p_rx trans : iProp Σ:=
-    ∃ ps_na' ps_acc' (trans' : gmap Word transaction) rx_state,
-               let ps_oea := ps_acc' ∖ {[p_rx;p_tx]} ∖ (pages_in_trans trans)  in
+  Definition vmprop_unknown_pre
+    (Φ: PID -d> PID -d> (gmap Word transaction) -d> iPropO Σ)
+    :PID -d> PID -d> (gmap Word transaction) -d> iPropO Σ :=
+    λ p_tx p_rx trans,
+    (∃ ps_na' ps_acc' (trans' : gmap Word transaction) rx_state,
+               let ps_macc_trans := (pages_in_trans (trans_memory_in_trans trans)) in
                let ps_macc_trans' := (pages_in_trans (trans_memory_in_trans trans')) in
-               let ps_oea' := ps_acc' ∖ {[p_rx;p_tx]} ∖ pages_in_trans trans' in
+               let ps_oea := ps_acc' ∖ {[p_rx;p_tx]} ∖ ps_macc_trans in
+               let ps_oea' := ps_acc' ∖ {[p_rx;p_tx]} ∖ ps_macc_trans' in
                (* lower bound *)
                i -@{1/2}A> ps_acc' ∗
                LB@ i := [ps_na'] ∗
@@ -134,7 +137,6 @@ Section logrel.
                (∃ mem_rx, memory_page p_rx mem_rx) ∗
                (* rx pages for all other VMs *)
                rx_pages (list_to_set (list_of_vmids) ∖ {[i]}) ∗
-               (* other RXs *)
                (* Implications: these implications relate [trans], the transactions at the beginning of the proof, and
                 [trans'], those at the point of switching to i. These assumptions are (I believe) necessary to prove FTLR.
                 Moreover, they are provable because of that fact that i as the invoker is the only vm can manipulate
@@ -150,12 +152,96 @@ Section logrel.
                ((∃ mem_oea, memory_pages ps_oea mem_oea) ∗ (∃ mem_trans, memory_transferred trans' mem_trans) -∗
                 ∃ mem_all, memory_pages (ps_acc' ∖ {[p_rx;p_tx]} ∪ ps_macc_trans') mem_all) ∗
                (* if i yielding, we give following resources back to pvm *)
-               VMProp V0 (vmprop_zero p_rx) (1/2)%Qp.
+               VMProp V0 (vmprop_zero_pre Φ p_tx p_rx) (1/2)%Qp)%I.
+
+  Local Instance vmprop_unknown_pre_contractive : Contractive (vmprop_unknown_pre).
+  Proof.
+  rewrite /vmprop_unknown_pre => n vmprop_unknown vmprop_unknown' Hvmprop_unknown p_tx p_rx trans /=.
+  f_equiv.
+    do 25 f_equiv.
+    rewrite /VMProp  /=.
+    do 6 f_equiv.
+    f_contractive.
+    rewrite /vmprop_zero_pre.
+    do 17 f_equiv.
+    rewrite /VMProp.
+    repeat f_equiv.
+    apply Hvmprop_unknown.
+Qed.
+
+  Definition vmprop_unknown:= fixpoint (vmprop_unknown_pre).
+
+  Definition vmprop_zero := vmprop_zero_pre vmprop_unknown.
+
+  Lemma vmprop_unknown_def : vmprop_unknown ≡
+     λ p_tx p_rx trans,
+      (∃ ps_na' ps_acc' (trans' : gmap Word transaction) rx_state,
+          let ps_macc_trans := (pages_in_trans (trans_memory_in_trans trans)) in
+          let ps_macc_trans' := (pages_in_trans (trans_memory_in_trans trans')) in
+          let ps_oea := ps_acc' ∖ {[p_rx;p_tx]} ∖ ps_macc_trans in
+          let ps_oea' := ps_acc' ∖ {[p_rx;p_tx]} ∖ ps_macc_trans' in
+          i -@{1/2}A> ps_acc' ∗
+          LB@ i := [ps_na'] ∗
+          ⌜ps_na' ## ps_acc' ∪ ps_macc_trans'⌝ ∗
+          transaction_hpool_global_transferred trans' ∗
+          transaction_pagetable_entries_transferred trans' ∗
+          retrieval_entries_transferred trans' ∗
+          (∃ mem_trans, memory_transferred trans' mem_trans) ∗
+          R0 @@ V0 ->r encode_hvc_func(Run) ∗ R1 @@ V0 ->r encode_vmid(i) ∗ (∃ r2, R2 @@ V0 ->r r2) ∗
+          RX_state@ i := rx_state ∗
+          (rx_page i p_rx) ∗
+          (∃ mem_rx, memory_page p_rx mem_rx) ∗
+          rx_pages (list_to_set (list_of_vmids) ∖ {[i]}) ∗
+          (transaction_pagetable_entries_owned trans -∗ transaction_pagetable_entries_owned trans') ∗
+          (pagetable_entries_excl_owned i ps_oea -∗ pagetable_entries_excl_owned i ps_oea') ∗
+          (retrieval_entries_owned trans -∗ retrieval_entries_owned trans') ∗
+          ((∃ mem_oea, memory_pages ps_oea mem_oea) ∗ (∃ mem_trans, memory_transferred trans' mem_trans) -∗
+          ∃ mem_all, memory_pages (ps_acc' ∖ {[p_rx;p_tx]} ∪ ps_macc_trans') mem_all) ∗
+          VMProp V0 (vmprop_zero p_tx p_rx) (1/2)%Qp)%I.
+  Proof.
+    rewrite /vmprop_unknown //.
+    rewrite (fixpoint_unfold vmprop_unknown_pre).
+    setoid_reflexivity.
+  Qed.
+
+  Global Instance vmprop_unknown_proper: Proper ((=) ==> (=) ==> (=) ==> (⊣⊢)) vmprop_unknown.
+  Proof. apply _. Qed.
+
+  Lemma vmprop_unknown_eq (p_tx p_rx:PID) (trans: gmap Word transaction): vmprop_unknown p_tx p_rx trans ⊣⊢
+      (∃ ps_na' ps_acc' (trans' : gmap Word transaction) rx_state,
+               let ps_macc_trans := (pages_in_trans (trans_memory_in_trans trans)) in
+               let ps_macc_trans' := (pages_in_trans (trans_memory_in_trans trans')) in
+               let ps_oea := ps_acc' ∖ {[p_rx;p_tx]} ∖ ps_macc_trans in
+               let ps_oea' := ps_acc' ∖ {[p_rx;p_tx]} ∖ ps_macc_trans' in
+               i -@{1/2}A> ps_acc' ∗
+               LB@ i := [ps_na'] ∗
+               ⌜ps_na' ## ps_acc' ∪ ps_macc_trans'⌝ ∗
+               transaction_hpool_global_transferred trans' ∗
+               transaction_pagetable_entries_transferred trans' ∗
+               retrieval_entries_transferred trans' ∗
+               (∃ mem_trans, memory_transferred trans' mem_trans) ∗
+               R0 @@ V0 ->r encode_hvc_func(Run) ∗ R1 @@ V0 ->r encode_vmid(i) ∗ (∃ r2, R2 @@ V0 ->r r2) ∗
+               RX_state@ i := rx_state ∗
+               (rx_page i p_rx) ∗
+               (∃ mem_rx, memory_page p_rx mem_rx) ∗
+               rx_pages (list_to_set (list_of_vmids) ∖ {[i]}) ∗
+               (transaction_pagetable_entries_owned trans -∗ transaction_pagetable_entries_owned trans') ∗
+               (pagetable_entries_excl_owned i ps_oea -∗ pagetable_entries_excl_owned i ps_oea') ∗
+               (retrieval_entries_owned trans -∗ retrieval_entries_owned trans') ∗
+               ((∃ mem_oea, memory_pages ps_oea mem_oea) ∗ (∃ mem_trans, memory_transferred trans' mem_trans) -∗
+                ∃ mem_all, memory_pages (ps_acc' ∖ {[p_rx;p_tx]} ∪ ps_macc_trans') mem_all) ∗
+               VMProp V0 (vmprop_zero p_tx p_rx) (1/2)%Qp)%I.
+    Proof.
+      rewrite /vmprop_unknown.
+      (* be patient, this line takes 30+ sec.. *)
+      apply (fixpoint_unfold vmprop_unknown_pre).
+    Qed.
 
   Program Definition interp_access p_tx p_rx ps_acc trans : iPropO Σ:=
     (
       (* exclusively owned pages are pages i has access to, but ain't in any transactions related to i. *)
-      let ps_oea := ps_acc ∖ {[p_rx;p_tx]} ∖ (pages_in_trans trans) in
+      let ps_macc_trans := (pages_in_trans (trans_memory_in_trans trans)) in
+      let ps_oea := ps_acc ∖ {[p_rx;p_tx]} ∖ ps_macc_trans in
       (* registers *)
       (∃ regs, ⌜is_total_gmap regs⌝ ∗ [∗ map] r ↦ w ∈ regs, r @@ i ->r w) ∗
       (* TX page and its memory *)
@@ -170,8 +256,37 @@ Section logrel.
       VMProp i (vmprop_unknown p_tx p_rx trans) (1/2)%Qp
     )%I.
 
+End logrel.
+
+Section logrel_prim.
+
+  Context `{hypconst:HypervisorConstants}.
+  Context `{hypparams:!HypervisorParameters}.
+  Context `{vmG: !gen_VMG Σ}.
+
+  Program Definition interp_access_prim p_tx p_rx ps_acc trans rx_state: iPropO Σ:=
+    (
+      let ps_macc_trans := (pages_in_trans (trans_memory_in_trans V0 trans)) in
+      let ps_oea := ps_acc ∖ {[p_rx;p_tx]} ∖ ps_macc_trans in
+      (∃ regs, ⌜is_total_gmap regs⌝ ∗ [∗ map] r ↦ w ∈ regs, r @@ V0 ->r w) ∗
+      (tx_page V0 p_tx ∗ ∃ mem_tx, memory_page p_tx mem_tx) ∗
+      V0 -@A> ps_acc ∗
+      ⌜{[p_tx;p_rx]} ⊆ ps_acc⌝ ∗
+      pagetable_entries_excl_owned V0 ps_oea ∗
+      transaction_pagetable_entries_owned V0 trans ∗ transaction_hpool_global_transferred trans ∗
+      transaction_pagetable_entries_transferred V0 trans ∗
+      retrieval_entries_owned V0 trans ∗ retrieval_entries_transferred V0 trans ∗
+      (∃ mem_oea, memory_pages ps_oea mem_oea) ∗ (∃ mem_trans, memory_transferred V0 trans mem_trans) ∗
+      RX_state@ V0 := rx_state ∗ (rx_page V0 p_rx) ∗
+      (∃ mem_rx, memory_page p_rx mem_rx) ∗
+      rx_pages (list_to_set (list_of_vmids) ∖ {[V0]}) ∗
+      VMProp V0 True 1%Qp ∗
+      [∗ set] i ∈ list_to_set (list_of_vmids) ∖ {[V0]}, VMProp (i:VMID) (vmprop_unknown i p_tx p_rx trans) (1/2)%Qp
+    )%I.
+
+End logrel_prim.
+
   (* Things we haven't really considerred:
    - [ ] if we need more pure propositions to relate trans'' and other stuff
    *)
 
-End logrel.
