theories/logrel/ftlr_reclaim.v
@@ -15,7 +15,6 @@ Section ftlr_reclaim.
 Lemma ftlr_reclaim {i trans' mem_acc_tx ai regs ps_acc p_tx p_rx ps_na instr trans rx_state r0}:
   base_extra.is_total_gmap regs ->
   {[p_tx; p_rx]} ⊆ ps_acc ->
-  i ≠ V0 ->
   ps_na ## ps_acc ∪ pages_in_trans (trans_memory_in_trans i trans) ->
   p_rx ∉ ps_acc ∖ {[p_rx; p_tx]} ∪ pages_in_trans (trans_memory_in_trans i trans) ->
   p_tx ∉ ps_acc ∖ {[p_rx; p_tx]} ∪ pages_in_trans (trans_memory_in_trans i trans) ->
@@ -34,8 +33,6 @@ Lemma ftlr_reclaim {i trans' mem_acc_tx ai regs ps_acc p_tx p_rx ps_na instr tra
           ⌜base_extra.is_total_gmap a⌝
             → ⌜{[p_tx; p_rx]} ⊆ a0⌝
               → ⌜ps_na ## a0 ∪ pages_in_trans (trans_memory_in_trans i a1)⌝
-                → ⌜p_rx ∉ a0 ∖ {[p_rx; p_tx]} ∪ pages_in_trans (trans_memory_in_trans i a1)⌝
-                  → ⌜p_tx ∉ a0 ∖ {[p_rx; p_tx]} ∪ pages_in_trans (trans_memory_in_trans i a1)⌝
                     → ([∗ map] r↦w ∈ a, r @@ i ->r w) -∗
                       TX@i:=p_tx -∗
                       p_tx -@O> - ∗ p_tx -@E> true -∗
@@ -51,7 +48,7 @@ Lemma ftlr_reclaim {i trans' mem_acc_tx ai regs ps_acc p_tx p_rx ps_na instr tra
                       RX_state@i:= a2 -∗
                       mailbox.rx_page i p_rx -∗
                       rx_pages (list_to_set list_of_vmids ∖ {[i]}) -∗
-                      ▷ VMProp V0 (vmprop_zero i p_rx) (1 / 2) -∗
+                      ▷ VMProp V0 (vmprop_zero i p_tx p_rx) (1 / 2) -∗
                       VMProp i (vmprop_unknown i p_tx p_rx trans') 1 -∗
                       transaction_pagetable_entries_owned i a1 -∗
                       pagetable_entries_excl_owned i (a0 ∖ {[p_rx; p_tx]} ∖ pages_in_trans a1) -∗
@@ -73,7 +70,7 @@ Lemma ftlr_reclaim {i trans' mem_acc_tx ai regs ps_acc p_tx p_rx ps_na instr tra
    RX_state@i:= rx_state -∗
    mailbox.rx_page i p_rx -∗
    rx_pages (list_to_set list_of_vmids ∖ {[i]}) -∗
-   ▷ VMProp V0 (vmprop_zero i p_rx) (1 / 2) -∗
+   ▷ VMProp V0 (vmprop_zero i p_tx p_rx) (1 / 2) -∗
    VMProp i (vmprop_unknown i p_tx p_rx trans') 1 -∗
    transaction_pagetable_entries_owned i trans -∗
    pagetable_entries_excl_owned i (ps_acc ∖ {[p_rx; p_tx]} ∖ pages_in_trans trans) -∗
@@ -83,7 +80,7 @@ Lemma ftlr_reclaim {i trans' mem_acc_tx ai regs ps_acc p_tx p_rx ps_na instr tra
    (∃ mem2 : mem, memory_page p_tx mem2) -∗
    SSWP ExecI @ i {{ bm, (if bm.1 then VMProp_holds i (1 / 2) else True) -∗ WP bm.2 @ i {{ _, True }} }}.
   Proof.
-    iIntros (Htotal_regs Hsubset_mb Hneq_0 Hdisj_na Hnin_rx Hnin_tx Hlookup_PC Hin_ps_acc Hneq_ptx Hdom_mem_acc_tx Hin_ps_acc_tx
+    iIntros (Htotal_regs Hsubset_mb Hdisj_na Hnin_rx Hnin_tx Hlookup_PC Hin_ps_acc Hneq_ptx Hdom_mem_acc_tx Hin_ps_acc_tx
                          Hlookup_mem_ai Heqn  Hlookup_reg_R0 Hdecode_hvc).
     iIntros (Hneq_mb) "IH regs tx pgt_tx pgt_acc pgt_acc' LB trans_hpool_global tran_pgt_transferred retri R0z R1z R2z rx_state rx other_rx prop0
              propi tran_pgt_owned pgt_owned retri_owned mem_rest mem_acc_tx mem_tx".
@@ -108,7 +105,7 @@ Lemma ftlr_reclaim {i trans' mem_acc_tx ai regs ps_acc p_tx p_rx ps_na instr tra
       iDestruct ("Hacc_mem_acc_tx" with "[$mem_instr]") as "mem_acc_tx".
       iDestruct (access_split with "pgt_acc") as "[pgt_acc pgt_acc']".
 
-      iApply ("IH" $! _ _ trans _ Htotal_regs' with "[] [] [] [] regs tx pgt_tx pgt_acc pgt_acc' LB [fresh_handles trans]
+      iApply ("IH" $! _ _ trans _ Htotal_regs' with "[] [] regs tx pgt_tx pgt_acc pgt_acc' LB [fresh_handles trans]
                             tran_pgt_transferred retri R0z R1z R2z rx_state rx other_rx prop0 propi tran_pgt_owned
                             pgt_owned retri_owned [mem_rest mem_acc_tx mem_tx]");auto.
       {
@@ -136,7 +133,7 @@ Lemma ftlr_reclaim {i trans' mem_acc_tx ai regs ps_acc p_tx p_rx ps_na instr tra
       iDestruct ("Hacc_mem_acc_tx" with "[$mem_instr]") as "mem_acc_tx".
       iDestruct (access_split with "pgt_acc") as "[pgt_acc pgt_acc']".
 
-      iApply ("IH" $! _ _ trans _ Htotal_regs' with "[] [] [] [] regs tx pgt_tx pgt_acc pgt_acc' LB [fresh_handles trans]
+      iApply ("IH" $! _ _ trans _ Htotal_regs' with "[] [] regs tx pgt_tx pgt_acc pgt_acc' LB [fresh_handles trans]
                             tran_pgt_transferred retri R0z R1z R2z rx_state rx other_rx prop0 propi tran_pgt_owned
                             pgt_owned retri_owned [mem_rest mem_acc_tx mem_tx]");auto.
       {
@@ -174,7 +171,7 @@ Lemma ftlr_reclaim {i trans' mem_acc_tx ai regs ps_acc p_tx p_rx ps_na instr tra
       iDestruct ("Hacc_mem_acc_tx" with "[$mem_instr]") as "mem_acc_tx".
       iDestruct (access_split with "pgt_acc") as "[pgt_acc pgt_acc']".
 
-      iApply ("IH" $! _ _ trans _ Htotal_regs' with "[] [] [] [] regs tx pgt_tx pgt_acc pgt_acc' LB [fresh_handles tran trans]
+      iApply ("IH" $! _ _ trans _ Htotal_regs' with "[] [] regs tx pgt_tx pgt_acc pgt_acc' LB [fresh_handles tran trans]
                             tran_pgt_transferred retri R0z R1z R2z rx_state rx other_rx prop0 propi tran_pgt_owned
                             pgt_owned retri_owned [mem_rest mem_acc_tx mem_tx]");auto.
       {
@@ -212,7 +209,7 @@ Lemma ftlr_reclaim {i trans' mem_acc_tx ai regs ps_acc p_tx p_rx ps_na instr tra
       iDestruct ("Hacc_mem_acc_tx" with "[$mem_instr]") as "mem_acc_tx".
       iDestruct (access_split with "pgt_acc") as "[pgt_acc pgt_acc']".
 
-      iApply ("IH" $! _ _ trans _ Htotal_regs' with "[] [] [] [] regs tx pgt_tx pgt_acc pgt_acc' LB [fresh_handles tran trans]
+      iApply ("IH" $! _ _ trans _ Htotal_regs' with "[] [] regs tx pgt_tx pgt_acc pgt_acc' LB [fresh_handles tran trans]
                             tran_pgt_transferred [re retri retri'] R0z R1z R2z rx_state rx other_rx prop0 propi tran_pgt_owned
                             pgt_owned retri_owned [mem_rest mem_acc_tx mem_tx]");auto.
       {
@@ -300,7 +297,7 @@ Lemma ftlr_reclaim {i trans' mem_acc_tx ai regs ps_acc p_tx p_rx ps_na instr tra
     iDestruct ("Hacc_mem_acc_tx" with "[$mem_instr]") as "mem_acc_tx".
     iDestruct (access_split with "pgt_acc") as "[pgt_acc pgt_acc']".
 
-    iApply ("IH" $! _ _ (delete r1 trans) _ Htotal_regs' with "[] [] [] [] regs tx pgt_tx pgt_acc pgt_acc' LB [fresh_handles trans]
+    iApply ("IH" $! _ _ (delete r1 trans) _ Htotal_regs' with "[] [] regs tx pgt_tx pgt_acc pgt_acc' LB [fresh_handles trans]
                             [tran_pgt_transferred] [retri retri'] R0z R1z R2z rx_state rx other_rx prop0 propi [tran_pgt_owned]
                             [own_tran excl_tran pgt_owned] [retri_owned] [mem_rest mem_acc_tx mem_tx]").
         {
@@ -313,20 +310,6 @@ Lemma ftlr_reclaim {i trans' mem_acc_tx ai regs ps_acc p_tx p_rx ps_na instr tra
           rewrite union_comm_L.
           rewrite union_assoc_L.
           set_solver + Hdisj_na Hsubseteq_tran.
-        }
-        {
-          iPureIntro.
-          rewrite Hrewrite.
-          rewrite union_comm_L.
-          rewrite difference_union_distr_l_L.
-          set_solver + Hdisj_na Hsubseteq_tran Hnin_rx.
-        }
-        {
-          iPureIntro.
-          rewrite Hrewrite.
-          rewrite union_comm_L.
-          rewrite difference_union_distr_l_L.
-          set_solver + Hdisj_na Hsubseteq_tran Hnin_tx.
         }
         {
           iExists (hpool ∪ {[r1]}).
@@ -443,7 +426,7 @@ Lemma ftlr_reclaim {i trans' mem_acc_tx ai regs ps_acc p_tx p_rx ps_na instr tra
     iDestruct ("Hacc_mem_acc_tx" with "[$mem_instr]") as "mem_acc_tx".
     iDestruct (access_split with "pgt_acc") as "[pgt_acc pgt_acc']".
 
-    iApply ("IH" $! _ _ (delete r1 trans) _ Htotal_regs' with "[] [] [] [] regs tx pgt_tx pgt_acc pgt_acc' LB [fresh_handles trans]
+    iApply ("IH" $! _ _ (delete r1 trans) _ Htotal_regs' with "[] [] regs tx pgt_tx pgt_acc pgt_acc' LB [fresh_handles trans]
                             [tran_pgt_transferred] [retri retri'] R0z R1z R2z rx_state rx other_rx prop0 propi [tran_pgt_owned]
                             [own_tran excl_tran pgt_owned] [retri_owned] [mem_rest mem_acc_tx mem_tx]").
         {
@@ -454,16 +437,6 @@ Lemma ftlr_reclaim {i trans' mem_acc_tx ai regs ps_acc p_tx p_rx ps_na instr tra
           iPureIntro.
           rewrite Hrewrite.
           set_solver + Hdisj_na Hsubseteq_tran.
-        }
-        {
-          iPureIntro.
-          rewrite Hrewrite.
-          set_solver + Hdisj_na Hsubseteq_tran Hnin_rx.
-        }
-        {
-          iPureIntro.
-          rewrite Hrewrite.
-          set_solver + Hdisj_na Hsubseteq_tran Hnin_tx.
         }
         {
           iExists (hpool ∪ {[r1]}).
@@ -579,7 +552,7 @@ Lemma ftlr_reclaim {i trans' mem_acc_tx ai regs ps_acc p_tx p_rx ps_na instr tra
     iDestruct ("Hacc_mem_acc_tx" with "[$mem_instr]") as "mem_acc_tx".
     iDestruct (access_split with "pgt_acc") as "[pgt_acc pgt_acc']".
 
-    iApply ("IH" $! _ _ (delete r1 trans) _ Htotal_regs' with "[] [] [] [] regs tx pgt_tx pgt_acc pgt_acc' LB [fresh_handles trans]
+    iApply ("IH" $! _ _ (delete r1 trans) _ Htotal_regs' with "[] [] regs tx pgt_tx pgt_acc pgt_acc' LB [fresh_handles trans]
                             [tran_pgt_transferred] [retri retri'] R0z R1z R2z rx_state rx other_rx prop0 propi [tran_pgt_owned]
                             [own_tran excl_tran pgt_owned] [retri_owned] [mem_rest mem_acc_tx mem_tx]").
         {
@@ -590,16 +563,6 @@ Lemma ftlr_reclaim {i trans' mem_acc_tx ai regs ps_acc p_tx p_rx ps_na instr tra
           iPureIntro.
           rewrite Hrewrite.
           set_solver + Hdisj_na Hsubseteq_tran.
-        }
-        {
-          iPureIntro.
-          rewrite Hrewrite.
-          set_solver + Hdisj_na Hsubseteq_tran Hnin_rx.
-        }
-        {
-          iPureIntro.
-          rewrite Hrewrite.
-          set_solver + Hdisj_na Hsubseteq_tran Hnin_tx.
         }
         {
           iExists (hpool ∪ {[r1]}).
