theories/logrel/ftlr_relinquish.v
@@ -15,7 +15,6 @@ Section ftlr_relinquish.
 Lemma ftlr_relinquish {i trans' mem_acc_tx ai regs ps_acc p_tx p_rx ps_na instr trans rx_state r0}:
   base_extra.is_total_gmap regs ->
   {[p_tx; p_rx]} ⊆ ps_acc ->
-  i ≠ V0 ->
   ps_na ## ps_acc ∪ pages_in_trans (trans_memory_in_trans i trans) ->
   p_rx ∉ ps_acc ∖ {[p_rx; p_tx]} ∪ pages_in_trans (trans_memory_in_trans i trans) ->
   p_tx ∉ ps_acc ∖ {[p_rx; p_tx]} ∪ pages_in_trans (trans_memory_in_trans i trans) ->
@@ -34,8 +33,6 @@ Lemma ftlr_relinquish {i trans' mem_acc_tx ai regs ps_acc p_tx p_rx ps_na instr 
           ⌜base_extra.is_total_gmap a⌝
             → ⌜{[p_tx; p_rx]} ⊆ a0⌝
               → ⌜ps_na ## a0 ∪ pages_in_trans (trans_memory_in_trans i a1)⌝
-                → ⌜p_rx ∉ a0 ∖ {[p_rx; p_tx]} ∪ pages_in_trans (trans_memory_in_trans i a1)⌝
-                  → ⌜p_tx ∉ a0 ∖ {[p_rx; p_tx]} ∪ pages_in_trans (trans_memory_in_trans i a1)⌝
                     → ([∗ map] r↦w ∈ a, r @@ i ->r w) -∗
                       TX@i:=p_tx -∗
                       p_tx -@O> - ∗ p_tx -@E> true -∗
@@ -51,7 +48,7 @@ Lemma ftlr_relinquish {i trans' mem_acc_tx ai regs ps_acc p_tx p_rx ps_na instr 
                       RX_state@i:= a2 -∗
                       mailbox.rx_page i p_rx -∗
                       rx_pages (list_to_set list_of_vmids ∖ {[i]}) -∗
-                      ▷ VMProp V0 (vmprop_zero i p_rx) (1 / 2) -∗
+                      ▷ VMProp V0 (vmprop_zero i p_tx p_rx) (1 / 2) -∗
                       VMProp i (vmprop_unknown i p_tx p_rx trans') 1 -∗
                       transaction_pagetable_entries_owned i a1 -∗
                       pagetable_entries_excl_owned i (a0 ∖ {[p_rx; p_tx]} ∖ pages_in_trans a1) -∗
@@ -73,7 +70,7 @@ Lemma ftlr_relinquish {i trans' mem_acc_tx ai regs ps_acc p_tx p_rx ps_na instr 
    RX_state@i:= rx_state -∗
    mailbox.rx_page i p_rx -∗
    rx_pages (list_to_set list_of_vmids ∖ {[i]}) -∗
-   ▷ VMProp V0 (vmprop_zero i p_rx) (1 / 2) -∗
+   ▷ VMProp V0 (vmprop_zero i p_tx p_rx) (1 / 2) -∗
    VMProp i (vmprop_unknown i p_tx p_rx trans') 1 -∗
    transaction_pagetable_entries_owned i trans -∗
    pagetable_entries_excl_owned i (ps_acc ∖ {[p_rx; p_tx]} ∖ pages_in_trans trans) -∗
@@ -83,7 +80,7 @@ Lemma ftlr_relinquish {i trans' mem_acc_tx ai regs ps_acc p_tx p_rx ps_na instr 
    (∃ mem2 : mem, memory_page p_tx mem2) -∗
    SSWP ExecI @ i {{ bm, (if bm.1 then VMProp_holds i (1 / 2) else True) -∗ WP bm.2 @ i {{ _, True }} }}.
   Proof.
-    iIntros (Htotal_regs Hsubset_mb Hneq_0 Hdisj_na Hnin_rx Hnin_tx Hlookup_PC Hin_ps_acc Hneq_ptx Hdom_mem_acc_tx Hin_ps_acc_tx
+    iIntros (Htotal_regs Hsubset_mb Hdisj_na Hnin_rx Hnin_tx Hlookup_PC Hin_ps_acc Hneq_ptx Hdom_mem_acc_tx Hin_ps_acc_tx
                          Hlookup_mem_ai Heqn  Hlookup_reg_R0 Hdecode_hvc).
     iIntros (Hneq_mb) "IH regs tx pgt_tx pgt_acc pgt_acc' LB trans_hpool_global tran_pgt_transferred retri R0z R1z R2z rx_state rx other_rx prop0
              propi tran_pgt_owned pgt_owned retri_owned mem_rest mem_acc_tx mem_tx".
@@ -107,7 +104,7 @@ Lemma ftlr_relinquish {i trans' mem_acc_tx ai regs ps_acc p_tx p_rx ps_na instr 
       iDestruct ("Hacc_mem_acc_tx" with "[$mem_instr]") as "mem_acc_tx".
       iDestruct (access_split with "pgt_acc") as "[pgt_acc pgt_acc']".
 
-      iApply ("IH" $! _ _ trans _ Htotal_regs' with "[] [] [] [] regs tx pgt_tx pgt_acc pgt_acc' LB [fresh_handles trans]
+      iApply ("IH" $! _ _ trans _ Htotal_regs' with "[] [] regs tx pgt_tx pgt_acc pgt_acc' LB [fresh_handles trans]
                             tran_pgt_transferred retri R0z R1z R2z rx_state rx other_rx prop0 propi tran_pgt_owned
                             pgt_owned retri_owned [mem_rest mem_acc_tx mem_tx]");auto.
       {
@@ -135,7 +132,7 @@ Lemma ftlr_relinquish {i trans' mem_acc_tx ai regs ps_acc p_tx p_rx ps_na instr 
       iDestruct ("Hacc_mem_acc_tx" with "[$mem_instr]") as "mem_acc_tx".
       iDestruct (access_split with "pgt_acc") as "[pgt_acc pgt_acc']".
 
-      iApply ("IH" $! _ _ trans _ Htotal_regs' with "[] [] [] [] regs tx pgt_tx pgt_acc pgt_acc' LB [fresh_handles trans]
+      iApply ("IH" $! _ _ trans _ Htotal_regs' with "[] [] regs tx pgt_tx pgt_acc pgt_acc' LB [fresh_handles trans]
                             tran_pgt_transferred retri R0z R1z R2z rx_state rx other_rx prop0 propi tran_pgt_owned
                             pgt_owned retri_owned [mem_rest mem_acc_tx mem_tx]");auto.
       {
@@ -173,7 +170,7 @@ Lemma ftlr_relinquish {i trans' mem_acc_tx ai regs ps_acc p_tx p_rx ps_na instr 
       iDestruct ("Hacc_mem_acc_tx" with "[$mem_instr]") as "mem_acc_tx".
       iDestruct (access_split with "pgt_acc") as "[pgt_acc pgt_acc']".
 
-      iApply ("IH" $! _ _ trans _ Htotal_regs' with "[] [] [] [] regs tx pgt_tx pgt_acc pgt_acc' LB [fresh_handles tran trans]
+      iApply ("IH" $! _ _ trans _ Htotal_regs' with "[] [] regs tx pgt_tx pgt_acc pgt_acc' LB [fresh_handles tran trans]
                             tran_pgt_transferred retri R0z R1z R2z rx_state rx other_rx prop0 propi tran_pgt_owned
                             pgt_owned retri_owned [mem_rest mem_acc_tx mem_tx]");auto.
       {
@@ -211,7 +208,7 @@ Lemma ftlr_relinquish {i trans' mem_acc_tx ai regs ps_acc p_tx p_rx ps_na instr 
       iDestruct ("Hacc_mem_acc_tx" with "[$mem_instr]") as "mem_acc_tx".
       iDestruct (access_split with "pgt_acc") as "[pgt_acc pgt_acc']".
 
-      iApply ("IH" $! _ _ trans _ Htotal_regs' with "[] [] [] [] regs tx pgt_tx pgt_acc pgt_acc' LB [fresh_handles tran trans]
+      iApply ("IH" $! _ _ trans _ Htotal_regs' with "[] [] regs tx pgt_tx pgt_acc pgt_acc' LB [fresh_handles tran trans]
                             tran_pgt_transferred [re retri retri'] R0z R1z R2z rx_state rx other_rx prop0 propi tran_pgt_owned
                             pgt_owned retri_owned [mem_rest mem_acc_tx mem_tx]");auto.
       {
@@ -289,7 +286,7 @@ Lemma ftlr_relinquish {i trans' mem_acc_tx ai regs ps_acc p_tx p_rx ps_na instr 
     iDestruct (access_split with "pgt_acc") as "[pgt_acc pgt_acc']".
     iDestruct (retri_split with "re") as "[re re']".
 
-    iApply ("IH" $! _ _ (<[r1 := ((tran.1, false):transaction)]> trans) _ Htotal_regs' with "[] [] [] [] regs tx pgt_tx pgt_acc
+    iApply ("IH" $! _ _ (<[r1 := ((tran.1, false):transaction)]> trans) _ Htotal_regs' with "[] [] regs tx pgt_tx pgt_acc
                             pgt_acc' LB [fresh_handles trans tran]
                             [tran_pgt_transferred] [retri retri' re re'] R0z R1z R2z rx_state rx other_rx prop0 propi [tran_pgt_owned]
                             [pgt_owned] [retri_owned] [mem_rest mem_acc_tx mem_tx]").
@@ -301,16 +298,6 @@ Lemma ftlr_relinquish {i trans' mem_acc_tx ai regs ps_acc p_tx p_rx ps_na instr 
       iPureIntro.
       rewrite Hrewrite.
       set_solver + Hdisj_na Hsubseteq_tran.
-    }
-    {
-      iPureIntro.
-      rewrite Hrewrite.
-      set_solver + Hdisj_na Hsubseteq_tran Hnin_rx.
-    }
-    {
-      iPureIntro.
-      rewrite Hrewrite.
-      set_solver + Hdisj_na Hsubseteq_tran Hnin_tx.
     }
     {
       iExists hpool.
