theories/logrel/ftlr_run.v
@@ -30,33 +30,33 @@ Lemma ftlr_run {i trans' mem_acc_tx ai regs ps_acc p_tx p_rx ps_na instr trans r
   decode_hvc_func r0 = Some Run ->
   p_tx ≠ p_rx ->
   ⊢
-  ▷ (∀ (a : gmap reg_name Addr) (a0 : gset PID) (a1 : gmap Addr transaction) (a2 : option (Addr * VMID)),
+  ▷ (∀ (a : gmap reg_name Addr) (a0 a1: gset PID) (a2 a3: gmap Addr transaction) (a4 : option (Addr * VMID)),
           ⌜base_extra.is_total_gmap a⌝
-            → ⌜{[p_tx; p_rx]} ⊆ a0⌝
-              → ⌜ps_na ## a0 ∪ pages_in_trans (trans_memory_in_trans i a1)⌝
-                → ⌜p_rx ∉ a0 ∖ {[p_rx; p_tx]} ∪ pages_in_trans (trans_memory_in_trans i a1)⌝
-                  → ⌜p_tx ∉ a0 ∖ {[p_rx; p_tx]} ∪ pages_in_trans (trans_memory_in_trans i a1)⌝
+            → ⌜{[p_tx; p_rx]} ⊆ a1⌝
+              → ⌜a0 ## a1 ∪ pages_in_trans (trans_memory_in_trans i a3)⌝
+                → ⌜p_rx ∉ a1 ∖ {[p_rx; p_tx]} ∪ pages_in_trans (trans_memory_in_trans i a3)⌝
+                  → ⌜p_tx ∉ a1 ∖ {[p_rx; p_tx]} ∪ pages_in_trans (trans_memory_in_trans i a3)⌝
                     → ([∗ map] r↦w ∈ a, r @@ i ->r w) -∗
                       TX@i:=p_tx -∗
                       p_tx -@O> - ∗ p_tx -@E> true -∗
-                      i -@{1 / 2}A> a0 -∗
-                      i -@{1 / 2}A> a0 -∗
-                      LB@ i := [ps_na] -∗
-                      transaction_hpool_global_transferred a1 -∗
-                      transaction_pagetable_entries_transferred i a1 -∗
-                      retrieval_entries_transferred i a1 -∗
+                      i -@{1 / 2}A> a1 -∗
+                      i -@{1 / 2}A> a1 -∗
+                      LB@ i := [a0] -∗
+                      transaction_hpool_global_transferred a3 -∗
+                      transaction_pagetable_entries_transferred i a3 -∗
+                      retrieval_entries_transferred i a3 -∗
                       R0 @@ V0 ->r encode_hvc_func Run -∗
                       R1 @@ V0 ->r encode_vmid i -∗
                       (∃ r2 : Addr, R2 @@ V0 ->r r2) -∗
-                      RX_state@i:= a2 -∗
+                      RX_state@i:= a4 -∗
                       mailbox.rx_page i p_rx -∗
                       rx_pages (list_to_set list_of_vmids ∖ {[i]}) -∗
-                      ▷ VMProp V0 (vmprop_zero i p_rx) (1 / 2) -∗
-                      VMProp i (vmprop_unknown i p_tx p_rx trans') 1 -∗
-                      transaction_pagetable_entries_owned i a1 -∗
-                      pagetable_entries_excl_owned i (a0 ∖ {[p_rx; p_tx]} ∖ pages_in_trans a1) -∗
-                      retrieval_entries_owned i a1 -∗
-                      (∃ mem : lang.mem, memory_pages (a0 ∪ pages_in_trans (trans_memory_in_trans i a1)) mem) -∗
+                      ▷ VMProp V0 (vmprop_zero i p_tx p_rx) (1 / 2) -∗
+                      VMProp i (vmprop_unknown i p_tx p_rx a2) 1 -∗
+                      transaction_pagetable_entries_owned i a3 -∗
+                      pagetable_entries_excl_owned i (a1 ∖ {[p_rx; p_tx]} ∖ (pages_in_trans (trans_memory_in_trans i a3))) -∗
+                      retrieval_entries_owned i a3 -∗
+                      (∃ mem : lang.mem, memory_pages (a1 ∪ pages_in_trans (trans_memory_in_trans i a3)) mem) -∗
                       WP ExecI @ i {{ _, True }}) -∗
    ([∗ map] r↦w ∈ regs, r @@ i ->r w) -∗
    TX@i:=p_tx -∗
@@ -73,10 +73,10 @@ Lemma ftlr_run {i trans' mem_acc_tx ai regs ps_acc p_tx p_rx ps_na instr trans r
    RX_state@i:= rx_state -∗
    mailbox.rx_page i p_rx -∗
    rx_pages (list_to_set list_of_vmids ∖ {[i]}) -∗
-   ▷ VMProp V0 (vmprop_zero i p_rx) (1 / 2) -∗
+   ▷ VMProp V0 (vmprop_zero i p_tx p_rx) (1 / 2) -∗
    VMProp i (vmprop_unknown i p_tx p_rx trans') 1 -∗
    transaction_pagetable_entries_owned i trans -∗
-   pagetable_entries_excl_owned i (ps_acc ∖ {[p_rx; p_tx]} ∖ pages_in_trans trans) -∗
+   pagetable_entries_excl_owned i (ps_acc ∖ {[p_rx; p_tx]} ∖ (pages_in_trans (trans_memory_in_trans i trans))) -∗
    retrieval_entries_owned i trans -∗
    (∃ mem1 : mem, memory_pages ((ps_acc ∪ (pages_in_trans (trans_memory_in_trans i trans))) ∖ ps_acc) mem1) -∗
    ([∗ map] k↦v ∈ mem_acc_tx, k ->a v) -∗
@@ -105,7 +105,7 @@ Lemma ftlr_run {i trans' mem_acc_tx ai regs ps_acc p_tx p_rx ps_na instr trans r
     iDestruct ("Hacc_mem_acc" with "[mem_instr]") as "mem"; iFrame.
     iAssert (memory_pages (ps_acc ∖ {[p_tx]}) _)%I with "[mem]" as "mem_acc".
     by iFrame.
-    iApply ("IH" $!  _ ps_acc trans _ Htotal_regs' Hsubset_mb Hdisj_na Hnin_rx Hnin_tx  with "regs tx pgt_tx pgt_acc pgt_acc'
+    iApply ("IH" $!  _ _ ps_acc _ trans _ Htotal_regs' Hsubset_mb Hdisj_na Hnin_rx Hnin_tx with "regs tx pgt_tx pgt_acc pgt_acc'
                  LB trans_hpool_global tran_pgt_transferred retri R0z R1z R2z rx_state rx other_rx prop0 propi tran_pgt_owned
                  pgt_owned retri_owned [mem_rest mem_acc mem_tx]").
     {
